examples/low-level/factorial.fst
@@ -1,10 +1,10 @@
 (*--build-config
 variables:LIB=../../lib;
-other-files:$LIB/ext.fst $LIB/set.fsi $LIB/set.fst $LIB/heap.fst $LIB/st.fst $LIB/all.fst $LIB/list.fst stack.fst listset.fst  $LIB/ghost.fst located.fst stackAndHeap.fst sst.fst sstCombinators.fst
+other-files:$LIB/ext.fst $LIB/set.fsi $LIB/set.fst $LIB/heap.fst $LIB/st.fst $LIB/all.fst $LIB/list.fst stack.fst listset.fst  $LIB/ghost.fst located.fst lref.fst stackAndHeap.fst sst.fst sstCombinators.fst
   --*)
 module Factorial
 open SSTCombinators
-open StackAndHeap  open Located
+open StackAndHeap  open Lref  open Located
 open SST
 open Heap
 open Stack
@@ -19,40 +19,40 @@ match n with
 | 0 -> 1
 | n -> n * factorial (n - 1)
 
-(* val factorialGuardLC :  n:nat -> li:(ref nat)  -> smem -> type *)
-type factorialGuardLC (n:nat) (li : ref nat) (m:smem) =
+(* val factorialGuardLC :  n:nat -> li:(lref nat)  -> smem -> type *)
+type factorialGuardLC (n:nat) (li : lref nat) (m:smem) =
   (refExistsInMem li m) && (not ((loopkupRef li m) = n))
 
-val factorialGuard :  n:nat -> li:(ref nat)  -> unit
+val factorialGuard :  n:nat -> li:(lref nat)  -> unit
   -> whileGuard (fun m -> b2t (refExistsInMem li m))
                 (factorialGuardLC n li)
 let factorialGuard n li u = not (memread li = n)
 (* the guard of a while loop is not supposed to change the memory*)
 
 
-type  loopInv (li : ref nat) (res : ref nat) (m:smem) =
+type  loopInv (li : lref nat) (res : lref nat) (m:smem) =
   refExistsInMem li m /\ refExistsInMem res m
     /\ (loopkupRef res m = factorial (loopkupRef li m))
     /\ (~ (li = res))
 
 open Ghost
 val factorialLoopBody :
-  n:nat -> li:(ref nat) -> res:(ref nat)
+  n:nat -> li:(lref nat) -> res:(lref nat)
   -> unit ->
   whileBody (loopInv li res) (factorialGuardLC n li)
   (hide (union (singleton (Ref li)) (singleton (Ref res))))
       (*SST unit (fun m -> loopInv li res (mtail m)) (fun m0 _ m1 -> loopInv li res (mtail m1))*)
-let factorialLoopBody (n:nat) (li:(ref nat)) (res:(ref nat)) u =
+let factorialLoopBody (n:nat) (li:(lref nat)) (res:(lref nat)) u =
   let liv = memread li in
   let resv = memread res in
   memwrite li (liv + 1);
   memwrite res ((liv+1) * resv)
  (*  (gunionUnion li res)*)
-val factorialLoop : n:nat -> li:(ref nat) -> res:(ref nat)
+val factorialLoop : n:nat -> li:(lref nat) -> res:(lref nat)
   -> Mem unit (fun m -> mreads li 0 m /\ mreads res 1 m  /\ ~(li=res))
               (fun m0 _ m1 -> mreads res (factorial n) m1)
               (hide (union (singleton (Ref li)) (singleton (Ref res))))
-let factorialLoop (n:nat) (li:(ref nat)) (res:(ref nat)) =
+let factorialLoop (n:nat) (li:(lref nat)) (res:(lref nat)) =
   scopedWhile
     (loopInv li res)
     (factorialGuardLC n li)
@@ -60,10 +60,10 @@ let factorialLoop (n:nat) (li:(ref nat)) (res:(ref nat)) =
     (hide (union (singleton (Ref li)) (singleton (Ref res))))
     (factorialLoopBody n li res)
 
-(*val factorialLoop2 : n:nat -> li:(ref nat) -> res:(ref nat)
+(*val factorialLoop2 : n:nat -> li:(lref nat) -> res:(lref nat)
   -> Mem unit (fun m -> mreads li 0 m /\ mreads res 1 m  /\ ~(li=res))
               (fun m0 _ m1 -> mreads res (factorial n) m1)
-let factorialLoop2 (n:nat) (li:(ref nat)) (res:(ref nat)) =
+let factorialLoop2 (n:nat) (li:(lref nat)) (res:(lref nat)) =
   scopedWhile1
     li
     (fun liv -> not (liv = 1))
@@ -93,8 +93,8 @@ let loopyFactorial2 n =
   #(fun _ rv _ -> rv == (factorial n)) (*this is the same as that of the conclusion, why cant it be inferred?*)
   #(hide empty)
   (fun u ->
-    let li:(ref nat) = salloc 0 in
-    let res:(ref nat) = salloc 1 in
+    let li:(lref nat) = salloc 0 in
+    let res:(lref nat) = salloc 1 in
     (scopedWhile1
       li
       (fun liv -> not (liv = n))
